WIP

code/ecdsap256/Hacl.Impl.P256.MixedPointAdd.fst
@@ -18,6 +18,8 @@ open Hacl.Impl.P256.LowLevel
 open Hacl.Impl.P256.PointAdd
 
 
+#set-options "--z3rlimit 100 --fuel 0 --ifuel 0"
+
 
 inline_for_extraction
 type pointAffine = lbuffer uint64 (size 8)
@@ -40,9 +42,50 @@ let pointAffineIsNotZero p =
   logor xZero yZero
 
 
+val copy_conditional_one_mm: out: felem -> mask: uint64 -> Stack unit
+  (requires fun h -> as_nat h out < prime256 /\ live h out /\ (uint_v mask == 0 \/ uint_v mask = pow2 64 - 1))
+  (ensures fun h0 _ h1 -> modifies (loc out) h0 h1 /\
+    as_nat h1 out < prime256 /\ (
+    if v mask = 0
+      then as_nat h1 out == as_nat h0 out
+      else 
+	as_nat h1 out == Spec.P256.MontgomeryMultiplication.toDomain_ 1  ))
+
+let copy_conditional_one_mm out mask = 
+  let out_0 = index out (size 0) in 
+  let out_1 = index out (size 1) in 
+  let out_2 = index out (size 2) in 
+  let out_3 = index out (size 3) in 
+
+  let x_0 = u64 1 in 
+  let x_1 = u64 18446744069414584320 in 
+  let x_2 = u64 18446744073709551615 in 
+  let x_3 = u64 4294967294 in 
+
+  let r_0 = logxor out_0 (logand mask (logxor out_0 x_0)) in 
+  let r_1 = logxor out_1 (logand mask (logxor out_1 x_1)) in 
+  let r_2 = logxor out_2 (logand mask (logxor out_2 x_2)) in 
+  let r_3 = logxor out_3 (logand mask (logxor out_3 x_3)) in 
+
+  lemma_xor_copy_cond out_0 x_0 mask;
+  lemma_xor_copy_cond out_1 x_1 mask;
+  lemma_xor_copy_cond out_2 x_2 mask;
+  lemma_xor_copy_cond out_3 x_3 mask;
+
+  upd out (size 0) r_0;
+  upd out (size 1) r_1;
+  upd out (size 2) r_2;
+  upd out (size 3) r_3;
+
+  Spec.P256.MontgomeryMultiplication.lemmaToDomain 1;
+  assert_norm(pow2 256 % prime256 = uint_v x_0 + uint_v x_1 * pow2 64 + uint_v x_2 * pow2 128 + uint_v x_3 * pow2 192);
+  assert_norm (pow2 64 * pow2 64 = pow2 128);
+  assert_norm (pow2 64 * pow2 64 * pow2 64 = pow2 192)
+
+
 val copy_point_conditional: out: point -> p: pointAffine -> maskPoint: point -> Stack unit 
   (requires fun h -> live h out /\ live h p /\ live h maskPoint /\ 
-    LowStar.Monotonic.Buffer.all_disjoint [loc p |+| loc out |+| loc maskPoint] /\
+    disjoint p out /\ disjoint p maskPoint /\ disjoint out maskPoint /\
     (
       let xOut = as_nat h (gsub out (size 0) (size 4)) in 
       let yOut = as_nat h (gsub out (size 4) (size 4)) in 
@@ -52,7 +95,27 @@ val copy_point_conditional: out: point -> p: pointAffine -> maskPoint: point -> 
       as_nat h (gsub p (size 4) (size 4)) < prime256
     )
   )
-  (ensures fun h0 _ h1 -> True) 
+  (ensures fun h0 _ h1 -> modifies (loc out) h0 h1 /\ (
+    let xOut = gsub out (size 0) (size 4) in 
+    let yOut = gsub out (size 4) (size 4) in 
+    let zOut = gsub out (size 8) (size 4) in 
+    as_nat h1 xOut < prime256 /\
+    as_nat h1 yOut < prime256 /\
+    as_nat h1 zOut < prime256 /\ (
+    
+    let mask = as_nat h0 (gsub maskPoint (size 8) (size 4)) in 
+    let x = gsub p (size 0) (size 4) in 
+    let y = gsub p (size 4) (size 4) in 
+
+    if mask = 0 then 
+      as_nat h1 xOut == as_nat h0 x /\ 
+      as_nat h1 yOut == as_nat h0 y /\ 
+      as_nat h1 zOut == Spec.P256.MontgomeryMultiplication.toDomain_ 1 
+    else 
+      as_nat h1 xOut == as_nat h0 xOut /\ 
+      as_nat h1 yOut == as_nat h0 yOut /\ 
+      as_nat h1 zOut == as_nat h0 zOut 
+    )))
 
 let copy_point_conditional out p maskPoint = 
   let z = sub maskPoint (size 8) (size 4) in 
@@ -67,8 +130,7 @@ let copy_point_conditional out p maskPoint =
 
   copy_conditional xOut p_x mask;
   copy_conditional yOut p_y mask;
-  (* 1 should be in Domaine*)
-  copy_conditional zOut (u64 1) mask
+  copy_conditional_one_mm zOut mask
 
 
 (* we except that we already know the q point *)
