code/ecdsap256/Hacl.P256.fst
@@ -83,3 +83,9 @@ let ecp256dh_r result pubKey scalar = Hacl.Impl.P256.DH.ecp256dh_r result pubKey
 let is_more_than_zero_less_than_order x =
   Hacl.Impl.P256.Signature.Common.isMoreThanZeroLessThanOrder x
  *) 
+
+
+
+
+
+ let pointAddMixed result p q =  Hacl.Impl.P256.MixedPointAdd.pointAddMixed result p q
